pico-ifc-coq/dyn_allocation/RefinementAC.v
@@ -37,9 +37,8 @@ Context {T: Type}
         {CLatt: ConcreteLattice T}
         {WFCLatt: WfConcreteLattice cblock T Latt CLatt}.
 
-Variable t1 : ASysTable T T.
-Variable t2 : ASysTable T unit.
-Hypothesis Ht1t2 : match_asystables t1 t2.
+Variable atable : ASysTable T.
+Hypothesis Hatable : parametric_asystable atable.
 
 Definition tini_fetch_rule_withsig :=
   (fun opcode => existT _
@@ -51,10 +50,10 @@ Definition tini_match_states := match_states cblock QuasiAbstractMachine.fetch_r
 Definition tini_concrete_machine := concrete_machine cblock tini_faultHandler.
 
 Program Definition abstract_concrete_ref :
-  refinement (abstract_machine t1) tini_concrete_machine :=
+  refinement (abstract_machine atable) tini_concrete_machine :=
   @ref_composition _ _ _
-                   (abstract_quasi_abstract_ref Ht1t2)
-                   (quasi_abstract_concrete_ref stamp_cblock fetch_rule t2)
+                   (abstract_quasi_abstract_ref Hatable)
+                   (quasi_abstract_concrete_ref stamp_cblock fetch_rule atable)
                    (@ac_match_initial_data _ _ _ _ fetch_rule)
                    match_events
                    _ _.
